\documentclass{article}
\usepackage{epsfig}
\pagestyle{empty}
\begin{document}
$ ( P_1, P_2) $
\pagebreak

\[ \frac {x - x_1 } {x_2 - x_1} = \frac { y - y_1 } {y_2 - y_1} = \frac { z - z_1 } {z_2 - z_1} \]
\pagebreak

$ a $
\pagebreak

\[ x = \left ( { \frac {\left ( \frac { ( B b + C c) x_0} {a} - B y_0 - C z_0 - D \right)} { ( A + B \frac {b} {a} + C \frac{c} {b})} }\right) \]
\pagebreak

\[ y = \left ( { \frac {\left ( C \frac {c}{b} y_0 - C z_0 - D \right)} { ( B + C \frac {c} {b}) } }\right) \]
\pagebreak

\[ z = \frac{c} {a} (x - x_0) + z_0 \]
\pagebreak

$ b $
\pagebreak

\[ x = x_0 \]
\pagebreak

\[ y = \frac{c} {b} (x - x_0) + y_0 \]
\pagebreak

\[ z = \frac{c} {b} (y - y_0) + z_0 \]
\pagebreak

\[ y = y_0 \]
\pagebreak

\[ z = \frac{(D + A x_0 + B y_0)} {C} \]
\pagebreak

$ (s, y, z) $
\pagebreak

$ (P_1, P_2) $
\pagebreak

\[ \frac {x - x_0 } {a} = \frac { y - y_0 } {b} = \frac { z - z_0 } {c} \]
\pagebreak

$ (x_0, y_0, z_0) $
\pagebreak

$ (a, b, c) $
\pagebreak

$ P $
\pagebreak

$ Ax + By + Cz + D = 0 $
\pagebreak

$ A, B $
\pagebreak

$ C $
\pagebreak

$ x, y $
\pagebreak

$ z $
\pagebreak

\end{document}
